\documentclass{article}
\title{Capítulo 10}
\author{Lucas Ferreira - 0418399}
\date{}
\usepackage{amsmath, graphicx, xcolor}

\begin{document}

\maketitle

\section{Exercícios 10.2}
1.
\begin{gather*}
    \int x \,dx
\\
    =\frac{x^2}{2} + k
\end{gather*}
2.
\begin{gather*}
    \int 3 \,dx
\\
    = 3x + k
\end{gather*}
3.
\begin{gather*}
    \int 3x + 1 \,dx
\\
    = \int 3x \,dx + \int 1 \,dx + k
\\
    = \frac{3x^2}{2} + k + x + k'
\\
    = \frac{3x^2}{2} + x + k
\end{gather*}
4.
\begin{gather*}
    \int (x^2 + x + 1) \,dx
\\
    = \int x^2 \,dx + \int x \,dx + \int 1 \,dx
\\
    = \frac{x^3}{3} +\frac{x^2}{2} + x + k
\end{gather*}
5.
\begin{gather*}
    \int x^3 \,dx
\\
    = \frac{x^4}{4} + k
\end{gather*}
6.
\begin{gather*}
    \int (x^3 + 2x + 3) \,dx
\\
    = \int x^3 \,dx + \int 2x \,dx + \int 3 \,dx
\\
    = \frac{x^4}{4} + 2\int x \,dx + 3x + k
\\
    = \frac{x^4}{4} + 2 * \frac{x^2}{2} + 3x + k
\\
    = \frac{x^4}{4} + x^2 + 3x + k
\end{gather*}
7.
\begin{gather*}
    \int \frac{1}{x^2} \,dx
\\
    = x^{-1}/-1 + k
\\
    = \frac{1}{x} * \frac{1}{-1} + k
\\
    = \frac{-1}{x} + k
\end{gather*}
8.
\begin{gather*}
    \int (x + \frac{1}{x^3}) \,dx
\\
    = \int x \,dx + \int \frac{1}{x^3} \,dx
\\
    = \frac{x^2}{2} + \frac{x^{-2}}{-2} + k
\\
    = \frac{x^2}{2} + \frac{1}{x^2} * \frac{1}{-2} + k
\\
    = \frac{x^2}{2} - \frac{1}{2x^2} + k
\end{gather*}
9.
\begin{gather*}
    \int \sqrt{x} \,dx
\\
    = \int x^\frac{1}{2} \,dx
\\
    = \frac{ \sqrt{x^3}}{\frac{3}{2}}
\\
    = \sqrt{x^3} * {\frac{2}{3}}
\\
    = \frac{2\sqrt{x^3}}{3} + k
\end{gather*}
10.
\begin{gather*}
    \int \sqrt[3]{x} \,dx
\\
    = \int x^\frac{1}{3} \,dx
\\
    = \frac{x^\frac{4}{3}}{\frac{4}{3}} + k
\\
    = \sqrt[3]{x^4} * \frac{3}{4}
\\
    = \frac{3\sqrt[3]{x^4}}{4} + k
\end{gather*}
11.
\begin{gather*}
    \int (x + \frac{1}{x}) \,dx
\\
    = \int x \,dx + \int \frac{1}{x} \,dx
\\
    = \frac{x^2}{2} + \ln x + k
\end{gather*}
12.
\begin{gather*}
    \int 2 + \sqrt[4]{x} \,dx
\\
    = \int 2 \,dx + \int \sqrt[4]{x} \,dx
\\
    = 2x + \int x^\frac{1}{4} \,dx
\\
    = 2x + \frac{x^\frac{1}{4}}{\frac{5}{4}} + k
\\
    = 2x + \frac{\sqrt[4]{x^5}}{\frac{5}{4}} + k
\\
    = 2x + \sqrt[4]{x^5} * \frac{4}{5} + k
\\
    = 2x + \frac{4\sqrt[4]{x^5}}{5} + k
\end{gather*}
13.
\begin{gather*}
    \int \sqrt{x} + \frac{1}{x^2} \,dx
\\
    = \int \sqrt{x} \,dx + \int \frac{1}{x^2} \,dx
\\
    = \frac{2\sqrt{x^3}}{3} + (-\frac{1}{x}) + k
\\
    = \frac{2\sqrt{x^3}}{3} - \frac{1}{x} + k
\\
\end{gather*}
14.
\begin{gather*}
    \int (\frac{2}{x} + \frac{3}{x^2}) \,dx
\\
    = 2 * \int \frac{1}{x} \,dx + 3 * \int \frac{1}{x^2} \,dx
\\
    = 2 \ln(x) + 3 * (\frac{-1}{x}) + k
\\
    = 2 \ln(x) + (\frac{-3}{x}) + k
\\
    = 2 \ln(x) - \frac{3}{x} + k
\\
\end{gather*}
15.
\begin{gather*}
    \int (2x^3 - \frac{1}{x^4}) \,dx
\\
    = 2 * \int x^3 \,dx - (\frac{-1}{3x^3}) + k
\\
    = \frac{x^4}{2} + \frac{1}{3x^3} + k
\\
\end{gather*}
16.
\begin{gather*}
    \int sen \alpha x \,dx
\\
    = \frac{1}{\alpha} \cos \alpha x + k
\\
    = \int sen u \frac{du}{\alpha} \
\\
    = \frac{1}{\alpha} \int sen u \,du
\\
    = -\frac{1}{\alpha} * (\cos u + k)
\\
    = -\frac{1}{\alpha} \cos \alpha x + k
\end{gather*}
17.
\begin{gather*}
    \int cos \alpha x \,dx
\\
    = \frac{1}{\alpha} sen \alpha x + k
\\
    = \int cos u \frac{du}{\alpha} \
\\
    = \frac{1}{\alpha} \int cos u \,du
\\
    = \frac{1}{\alpha} * (sen u + k)
\\
    = \frac{1}{\alpha} sen \alpha x + k
\end{gather*}
18.
\begin{gather*}
    \int e^{2x} \,dx
\\
    = \frac{1}{2} \int e^u \,du
\\
    = \frac{1}{2} * e^u + k
\\
    = \frac{e^{2x}}{2} + k
\end{gather*}
19.
\begin{gather*}
    \includegraphics[width=5cm]{19.png}
\end{gather*}
20.
\begin{gather*}
    \includegraphics[width=5cm]{20.png}
\end{gather*}


\end{document}
